src/study/Nemonuri.Study.CSharpSyntaxRewriter2.Modifier2/Nemonuri.StratifiedNodes.Forall.Children.fst
@@ -6,6 +6,8 @@ module C = Nemonuri.StratifiedNodes.Children
 module Common = Nemonuri.StratifiedNodes.Common
 module D = Nemonuri.StratifiedNodes.Decreasers
 module F = Nemonuri.StratifiedNodes.Factories
+open FStar.FunctionalExtensionality
+
 
 //--- theory members ---
 
@@ -19,46 +21,44 @@ let for_all_continue_predicate (t:eqtype)
   fun n v -> v
 
 
-let for_all_self_and_children #t
-  (parent:N.node t) 
-  (node_predicate:C.ancestor_list_given_selector t bool)
-  (ancestors:C.next_head_given_ancestor_list parent)
+let for_all_root_and_children #t
+  (root:N.node t) 
+  (node_predicate:N.node t -> bool)
   : Tot bool =
-  let node_predicate_for_child : (C.ancestor_list_given_selector_for_child t bool parent) = (
-    C.to_ancestor_list_given_selector_for_child t bool parent node_predicate
+  let selector : (C.ancestor_list_given_selector t bool) = (
+    C.to_ancestor_list_given_selector t bool node_predicate
+  ) in
+  let selector_for_child : (C.ancestor_list_given_selector_for_child t bool root) = (
+    C.to_ancestor_list_given_selector_for_child t bool root selector
   ) in
   C.select_and_aggregate_from_children 
-    parent node_predicate node_predicate_for_child
+    root selector selector_for_child
     for_all_aggregator
     for_all_aggregator
     (Common.aggregated_identity bool)
     (for_all_continue_predicate t)
-    ancestors
-    (N.get_children parent)
+    []
+    (N.get_children root)
     None
 
 //--- propositions ---
 
-let node1_satisfies_for_all_self_and_children_entails_node2_satisfies_predicate #t
+let node1_satisfies_for_all_root_and_children_entails_node2_satisfies_predicate #t
   (node1:N.node t) 
-  (node_predicate:C.ancestor_list_given_selector t bool)
-  (ancestors1:C.next_head_given_ancestor_list node1)
   (node2:N.node t)
-  (ancestors2:C.next_head_given_ancestor_list node2)
+  (node_predicate:N.node t -> bool)
   : prop =
-  ((for_all_self_and_children node1 node_predicate ancestors1) ==> 
-   (node_predicate node2 ancestors2))
+  ((for_all_root_and_children node1 node_predicate) ==> 
+   (node_predicate node2))
 
-let node_satisfies_for_all_self_and_children_entails_all_children_nodes_satisfy_predicate #t
+let node_satisfies_for_all_root_and_children_entails_all_children_nodes_satisfy_predicate #t
   (node:N.node t)
-  (node_predicate:C.ancestor_list_given_selector t bool)
-  (ancestors:C.next_head_given_ancestor_list node)
+  (node_predicate:N.node t -> bool)
   : prop =
   forall child_node. 
   (C.is_parent node child_node) ==>
-  (node1_satisfies_for_all_self_and_children_entails_node2_satisfies_predicate 
-    node node_predicate ancestors
-    child_node (C.concatenate_as_ancestor_list node ancestors)
+  (node1_satisfies_for_all_root_and_children_entails_node2_satisfies_predicate 
+    node child_node node_predicate
   )
 
 //---|
@@ -66,18 +66,34 @@ let node_satisfies_for_all_self_and_children_entails_all_children_nodes_satisfy_
 //--- proof ---
 
 let lemma1 #t
-  (parent:N.node t) 
-  (node_predicate:C.ancestor_list_given_selector t bool)
-  (ancestors:C.next_head_given_ancestor_list parent)
+  (root:N.node t) 
+  (node_predicate:N.node t -> bool)
   : Lemma
-    (requires (N.is_leaf parent))
+    (requires (N.is_leaf root) && (node_predicate root))
     (ensures 
-      node_satisfies_for_all_self_and_children_entails_all_children_nodes_satisfy_predicate
-        parent node_predicate ancestors
+      for_all_root_and_children root node_predicate
     )
   =
   ()
 
+#push-options "--query_stats"
+let lemma2 #t
+  (root:N.node t) 
+  (child:N.node t) 
+  (node_predicate:N.node t -> bool)
+  : Lemma
+    (requires 
+      (N.is_leaf child) && (node_predicate child) &&
+      (N.is_leaf root) &&
+      ( let root2 = D.prepend_child child root in
+        node_predicate root2 )
+    )
+    (ensures 
+      for_all_root_and_children root node_predicate
+    )
+  =
+  ()
+#pop-options 
 
 
 (*
